src/Serial.v
@@ -4,69 +4,32 @@ Require Import Common FMap Syntax Semantics.
 
 Section PerSystem.
   Variable sys: System.
-  Variable step: Step Msg.
+  Variable step: Step TState TLabel.
 
-  Record HLabel :=
-    { hlbl_hdl : Msg;
-      hlbl_outs : list Msg
-    }.
-
-  Definition toHLabel (l: Label): option HLabel :=
-    match l with
-    | LblHdl hdl outs => Some {| hlbl_hdl := hdl; hlbl_outs := outs |}
-    | _ => None
-    end.
-
-  Definition History := list HLabel.
-
-  Fixpoint historyOf (ll: list Label): History :=
-    match ll with
-    | nil => nil
-    | lbl :: ll' => (toHLabel lbl) ::> (historyOf ll')
-    end.
+  Definition History := list TLabel.
 
   Inductive HistoryOf: History -> Prop :=
   | Hist: forall ll st,
       steps step sys (getStateInit sys) ll st ->
-      HistoryOf (historyOf ll).
+      HistoryOf ll.
 
-  Inductive Atomic: Msg -> History -> list Msg -> Prop :=
+  Inductive Atomic: TMsg -> History -> list TMsg -> Prop :=
   | AtomicBase:
-      forall min hlbl mouts,
-        hlbl = {| hlbl_hdl := min; hlbl_outs := mouts |} ->
-        Atomic min (hlbl :: nil) mouts
+      forall min hlbl,
+        iLblHdl hlbl = Some min ->
+        Atomic min (hlbl :: nil) (iLblOuts hlbl)
   | AtomicCons:
       forall min hst mouts,
         Atomic min hst mouts ->
         forall hdl houts,
           In hdl mouts ->
-          Atomic min ({| hlbl_hdl := hdl; hlbl_outs := houts |} :: hst)
-                 (List.remove msg_dec hdl mouts ++ houts).
-
-  (* Definition isTrsPair (rq rs: MsgId) := *)
-  (*   (if mid_from rq ==n mid_to rs then true else false) *)
-  (*     && (if mid_to rq ==n mid_from rs then true else false) *)
-  (*     && (if mid_type rq ==n mid_type rs then true else false). *)
-
-  (* Definition AtomicTrs (hst: History) := *)
-  (*   exists min mout, *)
-  (*     isExternal sys (mid_from (msg_id min)) = true /\ *)
-  (*     isTrsPair (msg_id min) (msg_id mout) = true /\ *)
-  (*     Atomic min hst (mout :: nil). *)
-
-  (* Definition IncompleteTrs (hst: History) := *)
-  (*   exists min mouts, *)
-  (*     isExternal sys (mid_from (msg_id min)) = true /\ *)
-  (*     Forall (fun m => isInternal sys (mid_to (msg_id m)) = true) mouts /\ *)
-  (*     Atomic min hst mouts. *)
-
-  (* Definition Transactional (hst: History) := *)
-  (*   AtomicTrs hst \/ IncompleteTrs hst. *)
+          Atomic min (IlblInt (Some hdl) houts :: hst)
+                 (List.remove tmsg_dec hdl mouts ++ houts).
 
   Definition Transactional (hst: History) :=
     hst = nil \/
     (exists min mouts,
-        isExternal sys (mid_from (msg_id min)) = true /\
+        isExternal sys (mid_from (msg_id (tmsg_msg min))) = true /\
         Atomic min hst mouts).
 
   Definition Sequential (hst: History) :=
@@ -75,30 +38,21 @@ Section PerSystem.
 
 End PerSystem.
 
-Definition insOf (obj: Object) (hst: History) :=
-  filter (fun hl =>
-            if obj_idx obj ==n mid_from (msg_id (hlbl_hdl hl))
-            then true else false) hst.
-
-(* Two histories are equivalent if
- * 1) one history is a permutation of the other, and
- * 2) they have the same in-orders per an object.
- *)
-Definition Equivalent (hst1 hst2: History) :=
-  Permutation hst1 hst2 /\
-  forall obj, insOf obj hst1 = insOf obj hst2.
+Definition Equivalent {LabelT} `{HasLabel LabelT} (ll1 ll2: list LabelT) :=
+  Permutation ll1 ll2 /\ behaviorOf ll1 = behaviorOf ll2.
 
 Infix "≡" := Equivalent (at level 30).
 
-Definition Serializable (sys: System) (step: Step Msg) (ll: list Label) :=
+Definition Serializable {StateT} `{HasInit StateT}
+           (sys: System) (step: Step StateT TLabel) (ll: History) :=
   exists sll sst,
-    steps step sys (getStateInit sys) sll sst /\
-    Sequential sys (historyOf sll) /\
-    (* behaviorOf ll = behaviorOf sll /\ *)
-    Equivalent (historyOf ll) (historyOf sll).
+    (* 1) legal *) steps step sys (getStateInit sys) sll sst /\
+    (* 2) sequential *) Sequential sys sll /\
+    (* 3) equivalent *) ll ≡ sll.
 
 (* A system is [Serial] when all possible behaviors are [Serializable]. *)
-Definition Serial (sys: System) (step: Step Msg) :=
+Definition Serial {StateT} `{HasInit StateT}
+           (sys: System) (step: Step StateT TLabel) :=
   forall ll st,
     steps step sys (getStateInit sys) ll st ->
     Serializable sys step ll.
