src/SerialFacts.v
@@ -1,70 +1,8 @@
 Require Import Bool List String Peano_dec.
 Require Import Permutation.
-Require Import Common ListSupport FMap Syntax Semantics SemFacts SemDet SemSeq Serial.
+Require Import Common ListSupport FMap Syntax Semantics SemFacts StepDet StepSeq Serial.
 
 Set Implicit Arguments.
-
-Definition NonActive (ll: list Label) :=
-  Forall (fun l => match l with
-                   | LblHdl _ _ => False
-                   | _ => True
-                   end) ll.
-
-Lemma historyOf_nil:
-  forall ll,
-    historyOf ll = nil <-> NonActive ll.
-Proof.
-  unfold NonActive; intros; split.
-  - induction ll; intros; [auto|].
-    destruct a; simpl in H; [auto|auto|discriminate].
-  - induction ll; intros; [auto|].
-    inv H.
-    destruct a; simpl in *; intuition auto.
-Qed.
-
-Lemma historyOf_app:
-  forall ll hst1 hst2,
-    historyOf ll = hst1 ++ hst2 ->
-    exists ll1 ll2,
-      ll = ll1 ++ ll2 /\ historyOf ll1 = hst1 /\ historyOf ll2 = hst2.
-Proof.
-  induction ll; simpl; intros.
-  - apply eq_sym, app_eq_nil in H; dest; subst.
-    do 2 (exists nil); auto.
-  - destruct a; simpl in *.
-    + specialize (IHll _ _ H); dest; subst.
-      eexists (_ :: _), _; repeat split.
-    + specialize (IHll _ _ H); dest; subst.
-      eexists (_ :: _), _; repeat split.
-    + destruct hst1 as [|hst1].
-      * simpl in H; subst.
-        exists nil; eexists; repeat split.
-      * simpl in H; inv H.
-        specialize (IHll _ _ H2); dest; subst.
-        eexists (_ :: _), _; repeat split.
-Qed.
-
-Lemma nonActive_transactional:
-  forall sys ll,
-    NonActive ll -> Transactional sys (historyOf ll).
-Proof.
-  intros.
-  apply historyOf_nil in H.
-  rewrite H.
-  left; reflexivity.
-Qed.
-
-Lemma equiv_history_behavior:
-  forall sys lla sta llb stb,
-    steps step_mod sys (getStateInit sys) lla sta ->
-    steps step_mod sys (getStateInit sys) llb stb ->
-    historyOf lla ≡ historyOf llb ->
-    exists ll,
-      steps step_mod sys (getStateInit sys) ll stb /\
-      historyOf ll = historyOf llb /\
-      behaviorOf ll = behaviorOf lla.
-Proof.
-Admitted.
 
 Lemma transactional_cons_inv:
   forall sys a ll,
@@ -88,271 +26,15 @@ Proof.
   eauto using transactional_cons_inv.
 Qed.
 
-Lemma atm2Q_enq_comm:
-  forall am aa q,
-    atm2Q (enq {| atm_msg := am; atm_active := aa |} q) =
-    enq am (atm2Q q).
-Proof.
-  unfold atm2Q, enq; intros.
-  apply map_app.
-Qed.
-
-Lemma atm2Q_find:
-  forall chn cs,
-    (M.map atm2Q cs)@[chn] = cs@[chn] >>= (fun q => Some (atm2Q q)).
-Proof.
-  intros; rewrite M.F.P.F.map_o; reflexivity.
-Qed.
-
-Lemma atm2Q_deactivate:
-  forall q, atm2Q q = atm2Q (map deactivate q).
-Proof.
-  induction q; simpl; intros; auto.
-  rewrite IHq; reflexivity.
-Qed.
-
-Lemma atm2C_enqC_comm:
-  forall am aa chn cs,
-    atm2C (enqC chn {| atm_msg := am; atm_active := aa |} cs) =
-    enqC chn am (atm2C cs).
-Proof.
-  unfold atm2C, enqC; intros.
-  rewrite atm2Q_find.
-  destruct (cs@[chn]); simpl;
-    try (rewrite M.map_add, atm2Q_enq_comm; reflexivity).
-Qed.
-
-Lemma atm2C_find:
-  forall from mf,
-    (M.map atm2C mf)@[from] = mf@[from] >>= (fun cs => Some (atm2C cs)).
-Proof.
-  intros; rewrite M.F.P.F.map_o; reflexivity.
-Qed.
-
-Lemma atm2C_deactivateC:
-  forall cs, atm2C cs = atm2C (deactivateC cs).
-Proof.
-  unfold atm2C, deactivateC; intros.
-  M.ext chn.
-  do 2 rewrite atm2Q_find.
-  rewrite M.F.P.F.map_o.
-  destruct (cs@[chn]); simpl; [|reflexivity].
-  rewrite atm2Q_deactivate; reflexivity.
-Qed.
-
-Lemma atm2MF_enqMF_comm:
-  forall am aa from chn mf,
-    atm2MF (enqMF from chn {| atm_msg := am; atm_active := aa |} mf) =
-    enqMF from chn am (atm2MF mf).
-Proof.
-  unfold atm2MF, enqMF; intros.
-  rewrite atm2C_find.
-  destruct (mf@[from]); simpl.
-  - rewrite M.map_add, atm2C_enqC_comm; reflexivity.
-  - rewrite M.map_add, atm2C_enqC_comm.
-    unfold atm2C; rewrite M.map_empty; reflexivity.
-Qed.
-
-Lemma atm2MF_find:
-  forall to msgs,
-    (M.map atm2MF msgs)@[to] = msgs@[to] >>= (fun mf => Some (atm2MF mf)).
-Proof.
-  intros; rewrite M.F.P.F.map_o; reflexivity.
-Qed.
-
-Lemma atm2MF_deactivateMF:
-  forall mf, atm2MF mf = atm2MF (deactivateMF mf).
-Proof.
-  unfold atm2MF, deactivateMF; intros.
-  M.ext from.
-  do 2 rewrite atm2C_find.
-  rewrite M.F.P.F.map_o.
-  destruct (mf@[from]); simpl; [|reflexivity].
-  rewrite atm2C_deactivateC; reflexivity.
-Qed.
-
-Lemma atm2M_distributeMsg_comm:
-  forall am aa msgs,
-    atm2M (distributeMsg {| atm_msg := am; atm_active := aa |} msgs) =
-    distributeMsg am (atm2M msgs).
-Proof.
-  destruct am as [[mty mfr mto mch] mv]; intros.
-  unfold atm2M, distributeMsg, enqM; simpl.
-  rewrite atm2MF_find.
-  destruct (msgs@[mto]); simpl.
-  - rewrite M.map_add, atm2MF_enqMF_comm; reflexivity.
-  - rewrite M.map_add, atm2MF_enqMF_comm.
-    unfold atm2MF; rewrite M.map_empty; reflexivity.
-Qed.
-
-Lemma atm2M_deactivateM:
-  forall msgs, atm2M msgs = atm2M (deactivateM msgs).
-Proof.
-  unfold atm2M, deactivateM; intros.
-  M.ext to.
-  do 2 rewrite atm2MF_find.
-  rewrite M.F.P.F.map_o.
-  destruct (msgs@[to]); simpl; [|reflexivity].
-  rewrite atm2MF_deactivateMF; reflexivity.
-Qed.
-
-Lemma atm2M_distributeMsgs_active_comm:
-  forall ins msgs,
-    atm2M (distributeMsgs (toAtomicMsgsT ins) msgs) =
-    distributeMsgs ins (atm2M msgs).
-Proof.
-  induction ins; intros; [reflexivity|].
-  simpl; rewrite <-IHins.
-  apply atm2M_distributeMsg_comm.
-Qed.
-
-Lemma atm2M_distributeMsgs_inactive_comm:
-  forall ins msgs,
-    atm2M (distributeMsgs (toAtomicMsgsF ins) msgs) =
-    distributeMsgs ins (atm2M msgs).
-Proof.
-  induction ins; intros; [reflexivity|].
-  simpl; rewrite <-IHins.
-  apply atm2M_distributeMsg_comm.
-Qed.
-
-Lemma step_seq_ins:
-  forall sys ins st1 st2,
-    step_mod sys st1 (LblIns ins) st2 ->
-    forall ast1,
-      atm2State ast1 = st1 ->
-      exists ast2,
-        atm2State ast2 = st2 /\
-        step_seq sys ast1 (LblIns ins) ast2.
-Proof.
-  intros; subst.
-  apply step_mod_step_det in H.
-  inv H.
-
-  exists {| st_oss := st_oss ast1;
-            st_msgs := distributeMsgs (toAtomicMsgsF ins) (st_msgs ast1) |}.
-  split.
-  - unfold atm2State; simpl.
-    rewrite atm2M_distributeMsgs_inactive_comm.
-    reflexivity.
-  - destruct ast1 as [oss1 msgs1]; simpl.
-    econstructor; eauto.
-Qed.
-
-Lemma atomic_mouts_internal:
-  forall sys st1 ll st2,
-    steps step_mod sys st1 ll st2 ->
-    forall min mouts,
-      Atomic min (historyOf ll) mouts ->
-      Forall (fun m => isInternal sys (mid_from (msg_id m)) = true) mouts.
-Proof.
-  induction 1; simpl; intros; [inv H|].
-
-  destruct lbl; eauto.
-
-  simpl in H1; inv H1.
-  - inv H6.
-    apply step_mod_outs_internal in H0; auto.
-  - apply Forall_app.
-    + apply Forall_remove; eauto.
-    + apply step_mod_outs_internal in H0; auto.
-Qed.
-
-Lemma atomic_internals:
-  forall sys min mouts hll,
-    Atomic min hll mouts ->
-    forall ll st1 st2,
-      hll = historyOf ll ->
-      steps step_mod sys st1 ll st2 ->
-      Forall (fun hl => isInternal sys (mid_from (msg_id (hlbl_hdl hl))) = true)
-             (tl (rev hll)).
-Proof.
-  induction 1; simpl; intros; subst; [constructor|].
-
-  destruct hst as [|hl hst]; [constructor|].
-  rewrite tl_app by (simpl; destruct (rev hst); discriminate).
-
-  rewrite cons_app in H1.
-  apply eq_sym, historyOf_app in H1.
-  destruct H1 as [ll1 [ll2 [? [? ?]]]]; subst.
-
-  eapply steps_split in H2; [|reflexivity].
-  destruct H2 as [sti [? ?]].
-
-  apply Forall_app; eauto.
-
-  clear IHAtomic.
-  repeat constructor.
-  simpl.
-  rewrite <-H4 in H.
-  eapply atomic_mouts_internal in H1; [|eassumption].
-  eapply Forall_forall in H1; eauto.
-Qed.
-
-Lemma step_seq_hdl:
-  forall sys hdl outs ll,
-    Transactional sys ({| hlbl_hdl := hdl; hlbl_outs := outs |} :: historyOf ll) ->
-    forall ast1 ast2 st1 st2 st3,
-      atm2State ast1 = st1 ->
-      atm2State ast2 = st2 ->
-      steps step_mod sys st1 ll st2 ->
-      steps step_seq sys ast1 ll ast2 ->
-      step_mod sys st2 (LblHdl hdl outs) st3 ->
-      exists ast3,
-        atm2State ast3 = st3 /\
-        step_seq sys ast2 (LblHdl hdl outs) ast3.
-Proof.
-  intros; subst.
-  inv H; [discriminate|].
-  destruct H0 as [min [mouts [? ?]]].
-  destruct ast2 as [oss2 amsgs2].
-  apply step_mod_step_det in H4; inv H4.
-  exists {| st_oss := oss2 +[obj_idx obj <- pos];
-            st_msgs := distributeMsgs
-                         (toAtomicMsgsT (intOuts sys (pmsg_outs fpmsg os (msg_value hdl))))
-                         (if isExternal sys fidx then deactivateM amsgs2 else amsgs2) |}.
-  inv H0.
-
-  - inv H7.
-    split.
-    + unfold atm2State; simpl.
-      rewrite atm2M_distributeMsgs_active_comm.
-      destruct H13 as [? [? ?]]; subst.
-      rewrite H.
-      rewrite <-atm2M_deactivateM.
-      reflexivity.
-    + change min with (getMsg {| atm_msg := min; atm_active := false |}).
-      eapply SsInt; try reflexivity; try eassumption; eauto.
-      * destruct H13 as [? [? ?]]; subst; auto.
-      * admit.
-
-  - split.
-    + unfold atm2State; simpl.
-      rewrite atm2M_distributeMsgs_active_comm.
-      eapply atomic_mouts_internal in H9; [|eassumption].
-      eapply Forall_forall in H9; [|eassumption].
-      destruct H13 as [? [? ?]]; subst.
-      apply internal_not_external in H9; rewrite H9.
-      reflexivity.
-    + change hdl with (getMsg {| atm_msg := hdl; atm_active := true |}).
-      eapply SsInt; try reflexivity; try eassumption; eauto.
-
-      destruct ast1 as [oss1 amsgs1]; simpl in *.
-      unfold atm2State in H2; simpl in H2.
-      
-      admit.
-
-Admitted.
-
 Lemma transactional_steps_seq:
   forall sys ll,
-    Transactional sys (historyOf ll) ->
+    Transactional sys ll ->
     forall st1 st2,
-      steps step_mod sys st1 ll st2 ->
+      steps step_det sys st1 ll st2 ->
       forall ast1,
-        atm2State ast1 = st1 ->
+        at2TState ast1 = st1 ->
         exists ast2,
-          atm2State ast2 = st2 /\
+          at2TState ast2 = st2 /\
           steps step_seq sys ast1 ll ast2.
 Proof.
   induction ll as [|l ll]; simpl; intros; subst;
@@ -360,120 +42,113 @@ Proof.
 
   (* NOTE: [l] is the youngest label. *)
   inv H0.
-  specialize (IHll (transactional_ocons_inv _ _ H) _ _ H4 _ eq_refl).
+  specialize (IHll (transactional_cons_inv H) _ _ H4 _ eq_refl).
   destruct IHll as [past2 [? ?]]; subst.
-  destruct l; simpl in H.
-  - (* LblEmpty *)
-    apply step_mod_step_det in H6; inv H6.
-    eexists; repeat split.
-    econstructor; eauto.
-    econstructor.
-  - (* LblIns *)
-    eapply step_seq_ins in H6; [|reflexivity].
-    destruct H6 as [ast2 [? ?]]; subst.
-    eexists; repeat split.
-    econstructor; eauto.
-  - (* LblHdl *)
-    eapply step_seq_hdl in H; eauto.
-    destruct H as [ast3 [? ?]]; subst.
-    eexists; repeat split.
-    econstructor; eauto.
-Qed.
 
-Corollary nonActive_steps_seq:
-  forall ll,
-    NonActive ll ->
-    forall sys st1 st2,
-      steps step_mod sys st1 ll st2 ->
-      forall ast1,
-        atm2State ast1 = st1 ->
-        exists ast2,
-          atm2State ast2 = st2 /\
-          steps step_seq sys ast1 ll ast2.
-Proof.
-  intros.
-  apply nonActive_transactional with (sys:= sys) in H.
-  eauto using transactional_steps_seq.
-Qed.
+  destruct l.
+
+  - (* IlblExt *)
+    inv H; [discriminate|].
+    destruct H0 as [trin [trouts [? ?]]].
+    inv H6.
+    destruct past2 as [oss2 amsgs2 tid2 tcur2]; unfold at2TState in *; simpl in *.
+    eexists {| atst_cur := nts |}.
+
+    split; [reflexivity|].
+    econstructor; [eassumption|].
+    econstructor; eauto.
+
+  - (* IlblInt *)
+    inv H; [discriminate|].
+    destruct H0 as [trin [trouts [? ?]]].
+    inv H6; [inv H0; discriminate|].
+    destruct past2 as [oss2 amsgs2 tid2 tcur2]; unfold at2TState in *; simpl in *.
+    eexists {| atst_cur := tcur2 |}.
+
+    split; [reflexivity|].
+    econstructor; [eassumption|].
+    econstructor; eauto.
+
+    inv H0.
+    (* + exfalso. *)
+    (*   simpl in H7; inv H7. *)
+    (*   (* [fidx] should be an internal index *) *)
+    (* +  *)
+Admitted.
 
 Lemma sequential_steps':
   forall sys trs,
     Forall (Transactional sys) trs ->
     forall ll,
-      historyOf ll = concat trs ->
+      ll = concat trs ->
       forall st,
-        steps step_mod sys (getStateInit sys) ll st ->
+        steps step_det sys (getStateInit sys) ll st ->
         exists ast,
-          atm2State ast = st /\
+          at2TState ast = st /\
           steps step_seq sys (getStateInit sys) ll ast.
 Proof.
   induction trs; intros.
 
-  - simpl in H0; apply historyOf_nil in H0.
-    eapply nonActive_steps_seq; eauto.
-    unfold atm2State, atm2M, getStateInit; simpl.
-    mred.
+  - simpl in H0; subst.
+    inv H1.
+    exists (getStateInit sys); split.
+    + reflexivity.
+    + constructor.
 
   - inv H.
     specialize (IHtrs H5); clear H5.
 
-    simpl in H0.
-    apply historyOf_app in H0.
-    destruct H0 as [ll2 [ll1 [? [? ?]]]]; subst.
-
+    simpl in H1.
     eapply steps_split in H1; [|reflexivity].
     destruct H1 as [sti [? ?]].
-    specialize (IHtrs _ H2 _ H); clear H H2.
+    specialize (IHtrs _ eq_refl _ H); clear H.
     destruct IHtrs as [past [? ?]]; subst.
 
     pose proof (transactional_steps_seq H4 H0 eq_refl) as Hseq2.
     destruct Hseq2 as [ast2 [? ?]]; subst.
 
     eexists; split; [reflexivity|].
-    eauto using steps_append.
+    simpl; eauto using steps_append.
 Qed.
 
 Lemma sequential_steps:
   forall sys ll,
-    Sequential sys (historyOf ll) ->
+    Sequential sys ll ->
     forall st,
-      steps step_mod sys (getStateInit sys) ll st ->
+      steps step_det sys (getStateInit sys) ll st ->
       exists ast,
-        atm2State ast = st /\
+        at2TState ast = st /\
         steps step_seq sys (getStateInit sys) ll ast.
 Proof.
   unfold Sequential; intros.
-  destruct H as [trs [? ?]].
+  destruct H as [trs [? ?]]; subst.
   eauto using sequential_steps'.
 Qed.
 
 Theorem serializable_step_seq:
   forall sys ll st,
-    steps step_mod sys (getStateInit sys) ll st ->
-    Serializable sys step_mod ll ->
+    steps step_det sys (getStateInit sys) ll st ->
+    Serializable sys step_det ll ->
     Behavior step_seq sys (behaviorOf ll).
 Proof.
   unfold Serializable; intros.
   destruct H0 as [sll [sst [? [? ?]]]].
 
-  pose proof (equiv_history_behavior H H0 H2) as Hnll.
-  destruct Hnll as [nll [? [? ?]]].
-
-  rewrite <-H4 in H1.
-  pose proof (sequential_steps H1 H3) as Hseq.
+  pose proof (sequential_steps H1 H0) as Hseq.
   destruct Hseq as [ast [? ?]]; subst.
-
+  
   eapply Behv; eauto.
+  destruct H2; assumption.
 Qed.
 
 Theorem sequential_step_seq:
   forall sys,
-    Serial sys step_mod -> step_mod # step_seq |-- sys ⊑[id] sys.
+    Serial sys step_det -> step_det # step_seq |-- sys ⊑[id] sys.
 Proof.
   unfold Serial, Refines; intros.
-  rewrite map_id.
   inv H0; rename ll0 into ill. (* ill: the interleaving label sequence *)
   specialize (H _ _ H1).
+  rewrite map_id.
   eauto using serializable_step_seq.
 Qed.
 
