src/StepDet.v
@@ -1,0 +1,51 @@
+Require Import Bool List String Peano_dec.
+Require Import Common FMap Syntax Semantics.
+
+Inductive step_det (sys: System) : TState -> TLabel -> TState -> Prop :=
+| SdSlt: forall st, step_det sys st emptyILabel st
+| SdInt: forall ts oss oims obj idx os pos (fmsg: TMsg) fpmsg fidx fchn outs,
+    In obj (sys_objs sys) ->
+    idx = obj_idx obj ->
+    oss@[idx] = Some os ->
+
+    firstM fidx idx fchn oims = Some fmsg -> 
+    msg_id (getMsg fmsg) = pmsg_mid fpmsg ->
+    ValidMsgId fidx idx fchn fmsg ->
+    In fpmsg (obj_trs obj) ->
+    pmsg_precond fpmsg os ->
+    pmsg_postcond fpmsg os (msg_value (getMsg fmsg)) pos ->
+    outs = pmsg_outs fpmsg os (msg_value (getMsg fmsg)) ->
+    ValidOuts (obj_idx obj) outs ->
+
+    step_det sys
+             {| tst_oss := oss; tst_msgs := oims; tst_tid := ts |}
+             (IlblInt (Some fmsg) (extOuts sys (toTMsgs (tmsg_tid fmsg) outs)))
+             {| tst_oss := oss +[ idx <- pos ];
+                tst_msgs := distributeMsgs (intOuts sys (toTMsgs (tmsg_tid fmsg) outs)) oims;
+                tst_tid := ts
+             |}
+
+| SdExt: forall ts nts (Hts: nts > ts) oss oims obj os pos (emsg: Msg) fpmsg outs,
+    In obj (sys_objs sys) ->
+    oss@[obj_idx obj] = Some os ->
+
+    isExternal sys (mid_from (msg_id emsg)) = true ->
+    isInternal sys (mid_to (msg_id emsg)) = true ->
+
+    msg_id emsg = pmsg_mid fpmsg ->
+    In fpmsg (obj_trs obj) ->
+    pmsg_precond fpmsg os ->
+    pmsg_postcond fpmsg os (msg_value emsg) pos ->
+    outs = pmsg_outs fpmsg os (msg_value emsg) ->
+    ValidOuts (obj_idx obj) outs ->
+
+    step_det sys
+             {| tst_oss := oss; tst_msgs := oims; tst_tid := ts |}
+             (IlblExt {| tmsg_msg := emsg; tmsg_tid := ts |} (extOuts sys (toTMsgs ts outs)))
+             {| tst_oss := oss +[ obj_idx obj <- pos ];
+                tst_msgs := distributeMsgs (intOuts sys (toTMsgs ts outs)) oims;
+                tst_tid := nts
+             |}.
+
+Definition steps_det := steps step_det.
+
