src/StepSeq.v
@@ -1,0 +1,81 @@
+Require Import Bool List String Peano_dec.
+Require Import Permutation.
+Require Import Common FMap Syntax Semantics StepDet Serial.
+
+Record ATState : Type :=
+  { atst_oss : ObjectStates;
+    atst_msgs : Messages TMsg;
+    atst_tid : TrsId;
+    atst_cur : TrsId
+  }.
+
+Definition getATStateInit (sys: System): ATState :=
+  {| atst_oss := getObjectStatesInit (sys_objs sys);
+     atst_msgs := [];
+     atst_tid := trsIdInit;
+     atst_cur := trsIdInit
+  |}.
+
+Instance ATState_HasInit: HasInit ATState :=
+  { getStateInit := getATStateInit }.
+
+Definition at2TState (ats: ATState) :=
+  {| tst_oss := atst_oss ats;
+     tst_msgs := atst_msgs ats;
+     tst_tid := atst_tid ats |}.
+
+Inductive step_seq (sys: System) : ATState -> TLabel -> ATState -> Prop :=
+| SsSlt: forall st, step_seq sys st emptyILabel st
+| SsInt: forall ts cts oss oims obj idx os pos (fmsg: TMsg) fpmsg fidx fchn outs,
+    In obj (sys_objs sys) ->
+    idx = obj_idx obj ->
+    oss@[idx] = Some os ->
+
+    firstM fidx idx fchn oims = Some fmsg -> 
+    msg_id (getMsg fmsg) = pmsg_mid fpmsg ->
+    ValidMsgId fidx idx fchn fmsg ->
+    In fpmsg (obj_trs obj) ->
+    pmsg_precond fpmsg os ->
+    pmsg_postcond fpmsg os (msg_value (getMsg fmsg)) pos ->
+    outs = pmsg_outs fpmsg os (msg_value (getMsg fmsg)) ->
+    ValidOuts (obj_idx obj) outs ->
+
+    (* For internal steps, below is the only additional condition from [step_det]. *)
+    tmsg_tid fmsg = ts ->
+
+    step_seq sys
+             {| atst_oss := oss;
+                atst_msgs := oims;
+                atst_tid := ts;
+                atst_cur := cts |}
+             (IlblInt (Some fmsg) (extOuts sys (toTMsgs (tmsg_tid fmsg) outs)))
+             {| atst_oss := oss +[ idx <- pos ];
+                atst_msgs := distributeMsgs (intOuts sys (toTMsgs (tmsg_tid fmsg) outs)) oims;
+                atst_tid := ts;
+                atst_cur := cts |}
+
+| SsExt: forall ts cts nts (Hts: nts > ts) oss oims obj os pos (emsg: Msg) fpmsg outs,
+    In obj (sys_objs sys) ->
+    oss@[obj_idx obj] = Some os ->
+
+    isExternal sys (mid_from (msg_id emsg)) = true ->
+    isInternal sys (mid_to (msg_id emsg)) = true ->
+
+    msg_id emsg = pmsg_mid fpmsg ->
+    In fpmsg (obj_trs obj) ->
+    pmsg_precond fpmsg os ->
+    pmsg_postcond fpmsg os (msg_value emsg) pos ->
+    outs = pmsg_outs fpmsg os (msg_value emsg) ->
+    ValidOuts (obj_idx obj) outs ->
+
+    step_seq sys
+             {| atst_oss := oss;
+                atst_msgs := oims;
+                atst_tid := ts;
+                atst_cur := cts |}
+             (IlblExt {| tmsg_msg := emsg; tmsg_tid := ts |} (extOuts sys (toTMsgs ts outs)))
+             {| atst_oss := oss +[ obj_idx obj <- pos ];
+                atst_msgs := distributeMsgs (intOuts sys (toTMsgs ts outs)) oims;
+                atst_tid := nts;
+                atst_cur := nts |}.
+
